src/group/basic.lean
@@ -1,0 +1,322 @@
+import tactic
+
+/-!
+
+Basic definitions in group theory.
+
+Source: 
+https://xenaproject.wordpress.com/2018/04/30/group-theory-revision/
+
+-/
+
+set_option old_structure_cmd true -- it's better for this kind of stuff
+
+-- We're overwriting inbuilt group theory here so we always work in
+-- a namespace
+
+namespace mygroup
+
+-- definitions of the group classes
+
+section groupdefs 
+
+-- Set up notation typeclass using `extends`.
+class has_group_notation (G : Type) extends has_mul G, has_one G, has_inv G
+
+-- definition of the group structure
+class group (G : Type) extends has_group_notation G :=
+(mul_assoc : ∀ (a b c : G), a * b * c = a * (b * c))
+(one_mul : ∀ (a : G), 1 * a = a)
+(mul_left_inv : ∀ (a : G), a⁻¹ * a = 1)
+
+class comm_group (G : Type) extends group G :=
+(mul_comm : ∀ a b : G, a * b = b * a)
+
+-- an example
+instance perm_group (α : Type) : group (α ≃ α) :=
+{ mul := function.swap equiv.trans,
+  one := equiv.refl _,
+  inv := equiv.symm,
+  mul_assoc := by intros; ext; refl,
+  one_mul := by intros; ext; refl,
+  mul_left_inv := by intros; ext; simp }
+
+end groupdefs
+
+/- Our first task is to prove `mul_one` and `mul_right_inv`.
+   We prove some other things along the way too -- we make 
+   what a computer scientist would call "an interface for
+   the group class".
+
+  Examples of what we prove:
+
+`mul_left_cancel : ∀ (a b c : G), a * b = a * c → b = c`
+`mul_eq_of_eq_inv_mul {a x y : G} : x = a⁻¹ * y → a * x = y`
+`mul_one (a : G) : a * 1 = a`
+`mul_right_inv (a : G) : a * a⁻¹ = 1`
+
+-/
+namespace group
+
+variables {G : Type} [group G]  
+
+-- We prove left_mul_cancel for group using `calc`.
+
+lemma mul_left_cancel (a b c : G) (Habac : a * b = a * c) : b = c := 
+ calc b = 1 * b         : by rw one_mul
+    ... = (a⁻¹ * a) * b : by rw mul_left_inv
+    ... = a⁻¹ * (a * b) : by rw mul_assoc
+    ... = a⁻¹ * (a * c) : by rw Habac
+    ... = (a⁻¹ * a) * c : by rw mul_assoc
+    ... = 1 * c         : by rw mul_left_inv
+    ... = c             : by rw one_mul
+
+-- We can do all this one go:
+
+lemma mul_left_cancel' (a b c : G) (Habac : a * b = a * c) : b = c := 
+begin 
+  rw [←one_mul b, ←mul_left_inv a, mul_assoc, Habac,
+      ←mul_assoc, mul_left_inv, one_mul],
+end
+
+-- Because the above proof just uses one tactic, we could use `by`
+-- instead of `begin ... end`:
+
+lemma mul_left_cancel'' (a b c : G) (Habac : a * b = a * c) : b = c := 
+by rw [←one_mul b, ←mul_left_inv a, mul_assoc, Habac,
+  ←mul_assoc, mul_left_inv, one_mul]
+
+-- The below is also a useful intermediate lemma
+
+lemma mul_eq_of_eq_inv_mul {a x y : G} (h : x = a⁻¹ * y) : a * x = y :=
+begin
+  apply mul_left_cancel a⁻¹,
+  rw ←mul_assoc,
+  rw mul_left_inv,
+  rwa one_mul, -- rewrite then assumption
+end
+
+-- could prove it in `calc` mode:
+
+lemma mul_eq_of_eq_inv_mul' {a x y : G} (h : x = a⁻¹ * y) : a * x = y :=
+begin
+  apply mul_left_cancel a⁻¹,
+  exact calc
+  a⁻¹ * (a * x) = a⁻¹ * a * x : by rw mul_assoc
+  ...           = 1 * x       : by rw mul_left_inv
+  ...           = x           : by rw one_mul
+  ...           = a⁻¹ * y     : by rw h  
+end
+
+attribute [simp] one_mul mul_left_inv
+
+-- Alternatively, get the simplifier to do some of the work for us
+lemma mul_eq_of_eq_inv_mul'' {a x y : G} : x = a⁻¹ * y → a * x = y :=
+λ h, mul_left_cancel a⁻¹ _ _ $ by rw ←mul_assoc; simp [h]
+
+-- We can now prove `mul_one`:
+
+-- nice short proof
+theorem mul_one (a : G) : a * 1 = a :=
+begin
+  apply mul_eq_of_eq_inv_mul,
+  rw mul_left_inv,
+  -- note no refl
+end
+
+-- calc example (longer than previous one)
+theorem mul_one' : ∀ (a : G), a * 1 = a :=
+begin
+  intro a, -- goal is a * 1 = a
+  apply mul_left_cancel a⁻¹, -- goal now a⁻¹ * (a * 1) = a⁻¹ * a
+  exact calc a⁻¹ * (a * 1) = (a⁻¹ * a) * 1 : by rw mul_assoc
+          ...               = 1 * 1         : by rw mul_left_inv
+          ...               = 1             : by rw one_mul
+          ...               = a⁻¹ * a       : by rw mul_left_inv
+end
+
+-- term mode proof
+theorem mul_one'' (a : G) : a * 1 = a :=
+mul_eq_of_eq_inv_mul $ by simp
+
+-- it's also a good simp lemma
+attribute [simp] mul_one
+
+-- mul_left_inv is an axiom: here's mul_right_inv. 
+
+theorem mul_right_inv (a : G) : a * a⁻¹ = 1 :=
+begin
+  apply mul_eq_of_eq_inv_mul,
+  rw mul_one,
+end
+
+-- another good simp lemma
+attribute [simp] mul_right_inv
+
+-- We already proved `mul_eq_of_eq_inv_mul` but there are several other
+-- similar-looking, but slightly different, versions of this. Here
+-- is one.
+lemma eq_mul_inv_of_mul_eq {a b c : G} (h : a * c = b) : a = b * c⁻¹ :=
+begin
+  rw ←h,
+  rw mul_assoc,
+  rw mul_right_inv,
+  rw mul_one
+end
+
+-- one-liner proof
+lemma eq_mul_inv_of_mul_eq' {a b c : G} (h : a * c = b) : a = b * c⁻¹ :=
+by rw [←h, mul_assoc, mul_right_inv, mul_one]
+
+-- proof using automation
+lemma eq_mul_inv_of_mul_eq'' {a b c : G} (h : a * c = b) : a = b * c⁻¹ :=
+by simp [h.symm, mul_assoc]
+
+lemma eq_inv_mul_of_mul_eq {a b c : G} (h : b * a = c) : a = b⁻¹ * c :=
+begin
+  rw [←h, ←mul_assoc, mul_left_inv b, one_mul]
+end
+
+-- Another useful lemma for the interface:
+lemma mul_left_eq_self {a b : G} : a * b = b ↔ a = 1 :=
+begin
+  split,
+  { intro h,
+    replace h := eq_mul_inv_of_mul_eq h,
+    rw mul_right_inv at h,
+    assumption },
+  { intro h,
+    rw h,
+    rw one_mul }
+end
+
+lemma mul_right_eq_self {a b : G} : a * b = a ↔ b = 1 :=
+begin
+  split,
+    intro h,
+    from calc b = a⁻¹ * a : by apply eq_inv_mul_of_mul_eq h
+           ...  = 1 : by rw mul_left_inv,
+    intro h,
+    rw [h, mul_one]
+end
+
+-- Another useful lemma for the interface.
+-- Note use of the powerful `convert` tactic.
+-- `eq_mul_inv_of_mul_eq h` says ` a = 1 * b⁻¹` which is
+-- equal to our goal; convert creates the goals necessary
+-- to prove this
+lemma eq_inv_of_mul_eq_one {a b : G} (h : a * b = 1) : a = b⁻¹ :=
+begin
+  convert eq_mul_inv_of_mul_eq h,
+  rw one_mul, -- `simp` would also work
+end
+
+-- Another useful lemma for the interface
+lemma inv_inv (a : G) : a ⁻¹ ⁻¹ = a :=
+begin
+  symmetry,
+  apply eq_inv_of_mul_eq_one,
+  simp,
+end
+
+-- Another useful lemma for the interface
+lemma inv_eq_of_mul_eq_one {a b : G} (h : a * b = 1) : a⁻¹ = b :=
+begin
+  -- we can change hypotheses with the `replace` tactic.
+  -- h implies a = 1 * b⁻¹
+  replace h := eq_mul_inv_of_mul_eq h,
+  -- and so a = b⁻¹
+  rw one_mul at h,
+  -- By substituting in, we have to prove (b⁻¹)⁻¹ = b
+  rw h,
+  -- and we just did this, it's `inv_inv`
+  rw inv_inv,
+end
+
+lemma unique_id {e : G} (h : ∀ x : G, e * x = x) : e = 1 :=
+calc e = e * 1 : by rw mul_one
+  ...  = 1 : by rw h 1
+
+-- Maybe add unique_id but with x * e = x
+
+lemma unique_inv {a b : G} (h : a * b = 1) : b = a⁻¹ :=
+begin
+  apply mul_left_cancel a,
+  rw [h, mul_right_inv]
+end
+
+lemma mul_right_cancel (a x y : G) (Habac : x * a = y * a) : x = y := 
+calc x = x * 1 : by rw mul_one
+  ...  = x * (a * a⁻¹) : by rw mul_right_inv
+  ...  = x * a * a⁻¹ : by rw mul_assoc
+  ...  = y * a * a⁻¹ : by rw Habac
+  ...  = y * (a * a⁻¹) : by rw mul_assoc
+  ...  = y * 1 : by rw mul_right_inv
+  ...  = y : by rw mul_one
+
+lemma mul_left_cancel_iff (a x y : G) : a * x = a * y ↔ x = y :=
+begin
+  split,
+    from mul_left_cancel a x y,
+    intro hxy,
+    rwa hxy
+end
+
+lemma mul_right_cancel_iff (a x y : G) : x * a = y * a ↔ x = y :=
+begin
+  split,
+    from mul_right_cancel a x y,
+    intro hxy,
+    rwa hxy
+end
+
+@[simp] lemma inv_mul_cancel_left (a b : G) : a⁻¹ * (a * b) = b :=
+begin
+  rw ←mul_assoc, simp
+end
+
+@[simp] lemma mul_inv_cancel_left (a b : G) : a * (a⁻¹ * b) = b :=
+begin
+  rw ←mul_assoc,
+  simp
+end
+
+lemma inv_mul (a b : G) : (a * b)⁻¹ = b⁻¹ * a⁻¹ :=
+begin
+  apply mul_left_cancel (a * b),
+  rw mul_right_inv, simp [mul_assoc]
+end
+
+lemma one_inv : (1 : G)⁻¹ = 1 :=
+by conv_rhs { rw [←(mul_left_inv (1 : G)), mul_one] }
+
+attribute [simp] mul_left_cancel_iff mul_right_cancel_iff inv_mul inv_inv  one_inv
+
+@[simp] theorem inv_inj_iff {a b : G}: a⁻¹ = b⁻¹ ↔ a = b :=
+begin
+  split,
+  { intro h,
+    rw [← inv_inv a, h, inv_inv b] },
+  { rintro rfl,
+    refl }  
+end   
+
+theorem inv_eq {a b : G}: a⁻¹ = b ↔ b⁻¹ = a :=
+begin
+  split;
+  { rintro rfl,
+    rw inv_inv }
+end  
+
+-- **TODO** is this a good simp lemma? I don't think RHS is
+-- strictly simpler than LHS.
+@[simp] theorem mul_comm {G : Type} [comm_group G] (g h : G) : 
+  g * h = h * g := comm_group.mul_comm g h
+
+-- **TODO** open an issue about abel only working with `*`. We
+-- have `group` working but not `comm_group`. It
+-- would be an interesting exercise to get `abel` working.
+
+end group
+
+end mygroup
