src/orbit/basic.lean
@@ -1,0 +1,501 @@
+import subgroup.lagrange
+import data.nat.modeq
+
+noncomputable theory
+
+namespace mygroup
+
+open_locale classical
+
+open set classical function
+
+/-- A left action of some group `G` on some `S` is a function with type 
+  `to_fun : G → S → S` such that for all `s : S`, `to_fun 1 s = 1` and for all 
+  `g, h : G`, `s : S`, `to_fun g (to_fun h s) = to_fun (g * h) s` -/
+structure laction (G : Type) [group G] (S : Type) :=
+(to_fun    : G → S → S) (map_one' : ∀ s : S, to_fun 1 s = s)
+(map_assoc' : ∀ g h : G, ∀ s : S, to_fun g (to_fun h s) = to_fun (g * h) s)
+
+variables {G S : Type} [group G]
+variables {μ : laction G S}
+
+notation g ` •[`:70 μ `] `:0 s:70 := μ.to_fun g s
+local notation g ` • `:70  s:70  := μ.to_fun g s
+
+namespace laction
+
+-- APIs for left actions 
+
+@[ext] lemma ext (μ1 μ2 : laction G S)
+  (h : ∀ (g : G) (s : S), μ1.to_fun g s = μ2.to_fun g s) :
+μ1 = μ2 :=
+begin
+  cases μ1, cases μ2, simp * at *,
+  ext g s, apply h,
+end
+
+@[simp] lemma map_one (μ : laction G S) (s : S) : (1 •[μ] s) = s := μ.map_one' _
+
+lemma map_assoc (g h : G) (s : S) : g • (h • s) = g * h • s := 
+  μ.map_assoc' _ _ _
+
+-- The user should prove these two lemmas below
+
+lemma laction_mul_inv_cancel {g h : G} {s : S} : 
+  g • s = h • s ↔ s = (g⁻¹ * h) • s :=
+begin
+  split; intro hgh,
+    { conv_lhs { rw ←map_one μ s }, 
+      rw [←(group.mul_right_inv g⁻¹), ←map_assoc, 
+          ←map_assoc, ←hgh, group.inv_inv] },
+    { conv_lhs { rw [hgh, map_assoc, ←group.mul_assoc, 
+                     group.mul_right_inv, group.one_mul] } }
+end
+
+lemma laction_mul_inv {g : G} {s t : S} : g • s = t ↔ s = g⁻¹ • t :=
+begin
+  split; intro h,
+    { rw [←h, map_assoc, group.mul_left_inv, map_one] },
+    { rw [h, map_assoc, group.mul_right_inv, map_one] }
+end
+
+end laction
+
+/-- The orbit of some element of `s : S` is the image of the left action at `s` -/
+def orbit (μ : laction G S) (s : S) : set S := 
+  { m : S | ∃ g : G, m = g •[μ] s } 
+
+namespace laction
+
+@[simp]
+lemma orbit_def {s : S} : orbit μ s = { m : S | ∃ g : G, m = g • s } := rfl
+
+@[simp]
+lemma mem_orbit {s t : S} : t ∈ orbit μ s ↔ ∃ g : G, t = g • s := 
+by rw [orbit_def, mem_set_of_eq]
+
+/-- An element of `G` is in its own orbit -/
+lemma mem_orbit_refl (s : S) : s ∈ orbit μ s := ⟨1, (map_one μ s).symm⟩
+
+/-- If `s₁ : S` is in `s₂ : S`'s orbit, then `s₂` is in `s₁`'s orbit -/
+lemma mem_orbit_symm {s₁ s₂ : S} (h : s₁ ∈ orbit μ s₂) : s₂ ∈ orbit μ s₁ := 
+let ⟨g, hg⟩ := h in ⟨g⁻¹, by rw [hg, map_assoc, group.mul_left_inv, map_one]⟩
+
+/-- If s₁ ∈ [s₂] and s₂ ∈ [s₃] then s₁ ∈ [s₃] -/
+lemma mem_orbit_trans {s₁ s₂ s₃ : S} 
+  (hs₁ : s₁ ∈ orbit μ s₂) (hs₂ : s₂ ∈ orbit μ s₃) : s₁ ∈ orbit μ s₃ :=
+begin
+  cases hs₁ with g₁ hg₁,
+  cases hs₂ with g₂ hg₂,
+  refine ⟨g₁ * g₂, _⟩,
+  rw [hg₁, hg₂, map_assoc]
+end
+
+/-- If two elements of `S` are in the same orbit then they are in eachothers orbit-/
+lemma in_orbit_of_in_same_orbit {s₁ s₂ s₃ : S} 
+  (hs₁ : s₁ ∈ orbit μ s₃) (hs₂ : s₂ ∈ orbit μ s₃) : s₁ ∈ orbit μ s₂ :=
+begin
+  cases hs₁ with g₁ hg₁,
+  cases hs₂ with g₂ hg₂,
+  refine ⟨g₁ * g₂⁻¹, _⟩,
+  rw [hg₁, hg₂, map_assoc, group.mul_assoc, group.mul_left_inv, group.mul_one]
+end
+
+lemma in_orbit_of_inv' {s₁ s₂ : S} {g : G} (h : s₁ = g • s₂) : 
+  s₂ = g⁻¹ • s₁ := by rw [h, map_assoc, group.mul_left_inv, map_one]
+
+lemma eq_orbit {s₀ s₁ : S} (t : S) 
+  (hs₁ : t ∈ orbit μ s₀) (hs₂ : t ∈ orbit μ s₁) : orbit μ s₀ = orbit μ s₁ :=
+begin
+  cases hs₁ with g₁ hg₁,
+  cases hs₂ with g₂ hg₂,
+  ext, split; rintro ⟨g, rfl⟩,
+    { rw [hg₁, laction_mul_inv, map_assoc] at hg₂,
+      rw [mem_orbit, hg₂, map_assoc],
+      exact ⟨g * (g₁⁻¹ * g₂), rfl⟩ },
+    { rw [hg₂, laction_mul_inv, map_assoc] at hg₁,
+      rw [mem_orbit, hg₁, map_assoc],
+      exact ⟨g * (g₂⁻¹ * g₁), rfl⟩ } 
+end
+
+end laction
+
+/-- The stabilizer of `s : S` is the subgroup which elements fixes `s` under the 
+  left laction -/
+def stabilizer (μ : laction G S) (s : S) : subgroup G := 
+{ carrier := { g : G | (g •[μ] s) = s },
+  one_mem' := laction.map_one μ _,
+  mul_mem' := λ _ _ hg hh, 
+    by { rw mem_set_of_eq at *, rw [←laction.map_assoc, hh, hg] },
+  inv_mem' := λ x hx, 
+    begin
+      rw mem_set_of_eq at *, 
+      conv_lhs { rw ←hx },
+      rw [laction.map_assoc, group.mul_left_inv _, μ.2] 
+    end }
+
+/-- Two subgroups `H K` of group `G` are conjugates if and only if there exist 
+  some `g : G`, `g⁻¹ H g = K` -/
+def is_conjugate (H K : subgroup G) := 
+  ∃ g : G, { c | ∃ h ∈ H, c = g⁻¹ * h * g } = K
+
+-- This will be used in one of the lemmas later
+lemma nat.zero_or_one_of_le_one {n : ℕ} (hn : n ≤ 1) : n = 0 ∨ n = 1 := 
+begin
+  induction n, finish,
+  rw nat.succ_le_iff at hn,
+  change _ < 1 + 0 at hn,
+  rw nat.lt_one_add_iff at hn,
+  rw nat.le_zero_iff at hn,
+  right, rw hn,
+end
+
+namespace laction
+
+@[simp]
+lemma mem_stabilizer (s : S) (g : G) : g ∈ stabilizer μ s ↔ g • s = s := iff.rfl
+
+/-- If `H` is the conjugate of `K`, then `K` is the conjugate of `H` -/
+lemma is_conjugate_symm {H K : subgroup G} (h : is_conjugate H K) :
+  is_conjugate K H := 
+begin
+  cases h with g hg, refine ⟨g⁻¹, _⟩,
+  ext, split; intro hx, 
+    { rcases hx with ⟨h, hh₀, hh₁⟩,
+      change h ∈ (K : set G) at hh₀,
+      rw ←hg at hh₀,
+      rcases hh₀ with ⟨k, hk₀, hk₁⟩,
+      rw [hh₁, hk₁], simpa [group.mul_assoc] },
+    { rw mem_set_of_eq,
+      refine ⟨g⁻¹ * x * g, _, by simp [group.mul_assoc]⟩,
+      show g⁻¹ * x * g ∈ (K : set G),
+      rw ←hg, exact ⟨x, hx, rfl⟩ }
+end
+
+/-- If two elements are in the same orbit, then their stabilizers are conjugates -/
+theorem conjugate_stabilizer_of_in_same_orbit {s₁ s₂ s₃ : S} 
+  (hs₁ : s₁ ∈ orbit μ s₃) (hs₂ : s₂ ∈ orbit μ s₃) : 
+  is_conjugate (stabilizer μ s₁) (stabilizer μ s₂) :=
+begin
+  cases in_orbit_of_in_same_orbit hs₁ hs₂ with g hg,
+  refine ⟨g, _⟩,
+  ext, split; intro hx,
+    { show x ∈ stabilizer μ s₂,
+      rcases hx with ⟨h, hh₀, hh₁⟩,
+      rw [mem_stabilizer, hh₁, ←map_assoc, ←map_assoc, ←hg, 
+         (show h • s₁ = s₁, by exact hh₀), hg, map_assoc, 
+         group.mul_left_inv, map_one] },
+    { change x ∈ stabilizer μ s₂ at hx, 
+      refine ⟨g * x * g⁻¹, (mem_stabilizer _ _).2 _, _⟩,
+      rw [←map_assoc, ←(in_orbit_of_inv' hg), 
+          ←map_assoc, (mem_stabilizer _ _).1 hx, hg], by simp [group.mul_assoc] }
+end
+
+private structure extract_struct {μ : laction G S} {a : S} (s : orbit μ a) :=
+(val : G) (prop : s.1 = μ.to_fun val a)
+
+@[reducible] private def extract {μ : laction G S} {a : S} (s : orbit μ a) : 
+  extract_struct s := ⟨some s.2, some_spec s.2⟩
+
+@[reducible] private def aux_map (μ : laction G S) (a : S) : 
+  orbit μ a → { s | ∃ h : G, s = h ⋆ stabilizer μ a } := 
+λ s, ⟨(extract s).1 ⋆ stabilizer μ a, (extract s).1, rfl⟩
+
+private lemma aux_map_biject {a : S} : bijective $ aux_map μ a :=
+begin
+  split,
+    { rintro ⟨x, hx⟩ ⟨y, hy⟩ hxy,
+      rw [subtype.mk.inj_eq, lagrange.lcoset_eq] at hxy,
+      change ((extract ⟨y, hy⟩).val)⁻¹ * (extract ⟨x, hx⟩).val ∈ 
+        { g : G | g • a = a } at hxy,
+      rw [mem_set_of_eq, ←μ.3, ←(extract ⟨x, hx⟩).2, 
+        @laction_mul_inv _ _ _ μ _ x a, group.inv_inv, ←(extract ⟨y, hy⟩).2] at hxy,
+      simp only [hxy] },
+    { rintro ⟨_, g, hg⟩, refine ⟨⟨g • a, g, rfl⟩, _⟩,
+      rw [subtype.mk.inj_eq, hg, lagrange.lcoset_eq],
+      show g⁻¹ * (extract ⟨μ.to_fun g a, _⟩).val ∈ { g : G | g • a = a },
+      rw [mem_set_of_eq, ←μ.3, ←(extract ⟨μ.to_fun g a, _⟩).2, 
+        μ.3, group.mul_left_inv, μ.2] }
+end 
+
+-- With this function defined, we see that the cardinality of orbit s equals 
+-- the number of left cosets of stabilizer s
+
+lemma card_orbit_eq_num_lcoset {a : S} : 
+  fincard' (orbit μ a) = fincard' { s | ∃ h : G, s = h ⋆ stabilizer μ a } :=
+fincard.of_equiv (equiv.of_bijective _ aux_map_biject)
+
+/-- Orbit-Stabilizer : The cardinality of a finite group `G` given a laction `μ` 
+on some `S` equals the cardinality of the orbit of `s` multiplied by the 
+cardinality of the stabilizer of `s` for any `s : S` -/
+theorem orbit_stabilizer [h: fintype G] {a : S} (μ : laction G S) : 
+  fincard' G = fincard' (orbit μ a) * fincard' (stabilizer μ a) := 
+by rw [card_orbit_eq_num_lcoset, mul_comm]; exact lagrange.lagrange 
+
+/-! # fixed points -/
+
+end laction
+
+def fixed_points (μ : laction G S) : set S := { s : S | ∀ g : G, g •[μ] s = s }
+
+@[simp] lemma mem_fixed_points_iff (s : S) :
+  s ∈ fixed_points μ ↔ ∀ (g : G) , g • s = s := iff.rfl
+
+lemma mem_fixed_points_iff_stabilizer_univ (s : S) :
+  s ∈ fixed_points μ ↔ stabilizer μ s = ⊤ :=
+begin
+  rw mem_fixed_points_iff,
+  rw subgroup.eq_top_iff',
+  apply forall_congr,
+  intro a, refl
+end
+
+lemma orbit_eq_singleton {s : S} {μ : laction G S} (h : s ∈ fixed_points μ) : 
+  orbit μ s = {s} := by ext x; simp * at *
+
+lemma mem_fixed_points {s : S} {μ : laction G S} (h : orbit μ s = {s}) :
+  s ∈ fixed_points μ := λ k, mem_singleton_iff.1 begin exact h ▸ ⟨k, rfl⟩ end
+
+lemma orbit_eq_singleton_iff {s : S} {μ : laction G S} :
+  orbit μ s = {s} ↔ s ∈ fixed_points μ := ⟨mem_fixed_points, orbit_eq_singleton⟩
+
+lemma mem_fixed_points_iff_card_orbit_eq_one {s : S} {μ : laction G S}:
+  s ∈ fixed_points μ ↔ fincard' (orbit μ s) = 1 :=
+begin
+  rw ← orbit_eq_singleton_iff,
+  split; intro h,
+    { simp [h] },
+    { rw eq_singleton_iff_unique_mem,
+      refine ⟨laction.mem_orbit_refl _, λ y hy, _⟩,
+      rcases fincard.card_eq_one_iff_singleton.1 h with ⟨x, hx⟩, 
+      rw hx at hy,
+      rw [mem_singleton_iff.1 hy, ← mem_singleton_iff, ← hx],
+      exact laction.mem_orbit_refl _ }
+end
+
+-- should now prove that for G acting on S, size of S = sum
+-- of size of orbits.
+
+/-- Orbits of an action -/
+def orbits (μ : laction G S) := setoid.classes
+  { r := λ (x y : S), x ∈ orbit μ y,
+    iseqv := ⟨laction.mem_orbit_refl,
+            λ x y, laction.mem_orbit_symm,
+            λ x y z, laction.mem_orbit_trans⟩ }
+
+lemma orbit_mem_orbits (s : S) : orbit μ s ∈ orbits μ := ⟨s, rfl⟩
+
+lemma orbit_unique {x : S} {s : set S} (hs : s ∈ orbits μ) : 
+  x ∈ s ↔ orbit μ x = s :=
+begin
+  unfold orbits at hs,
+  change s ∈ {s | ∃ y, s = {x | x ∈ orbit μ y}} at hs,
+  rcases hs with ⟨y, rfl⟩,
+  split; intro hx,
+    { change x ∈ orbit μ y at hx,
+      exact laction.eq_orbit x (laction.mem_orbit_refl _) hx },
+    { change orbit μ x = orbit μ y at hx,
+      rw ←hx, exact laction.mem_orbit_refl _ }
+end
+
+lemma sum_card_orbits [fintype S] : ∑' o in (orbits μ), fincard' o = fincard' S :=
+  (fincard.card_eq_finsum_partition (setoid.is_partition_classes _)).symm
+
+lemma card_orbits_eq_one [fintype S] {s : set S} 
+  (hs₀ : s ∈ orbits μ) (hs₁ : fincard' s ≤ 1) : fincard' s = 1 :=
+begin
+  cases nat.zero_or_one_of_le_one hs₁,
+    { change s ∈ {s | ∃ y, s = {x | x ∈ orbit μ y}} at hs₀,
+      rcases hs₀ with ⟨x, hx⟩,
+      change s = orbit μ x at hx,
+      rw fincard.card_eq_zero_iff at h,
+      exfalso,
+      apply not_mem_empty x,
+      rw [←h, hx],
+      exact laction.mem_orbit_refl x },
+    { assumption }
+end
+
+def map_singleton (μ : laction G S) : (fixed_points μ) → 
+  ({o ∈ orbits μ | fincard' o ≤ 1} : set (set S)) :=
+λ s, ⟨orbit μ s, orbit_mem_orbits _,
+  let ⟨_, hs⟩ := s in le_of_eq (mem_fixed_points_iff_card_orbit_eq_one.1 hs)⟩
+
+@[simp] lemma map_singleton_def (s : S) (hs : s ∈ fixed_points μ) : 
+  (map_singleton μ ⟨s, hs⟩ : set S) = {s} :=
+begin
+  suffices : {m : S | ∃ (g : G), m = g • s} = {s},
+    simpa [map_singleton], 
+  finish,
+end
+
+lemma bijective_map_singleton [fintype S] (μ : laction G S) : 
+  function.bijective (map_singleton μ) :=
+begin
+  split,
+    { rintros ⟨x, hx⟩ ⟨y, hy⟩ hxy, congr,
+      rw ←singleton_eq_singleton_iff,
+      iterate 2 { rw ←map_singleton_def _ }, rw hxy },
+    { rintros ⟨y, hy₀, hy₁⟩,
+      rcases fincard.card_eq_one_iff_singleton.1 
+        (card_orbits_eq_one hy₀ hy₁) with ⟨x, rfl⟩,
+      refine ⟨⟨x, _⟩, _⟩,
+        { rw ←orbit_eq_singleton_iff,
+          exact (orbit_unique hy₀).1 (mem_singleton _) },
+        { suffices : {m : S | ∃ (g : G), m = g • x} = {x},
+            simpa [map_singleton],
+          suffices : x ∈ fixed_points μ,
+            finish,
+          rw ←orbit_eq_singleton_iff,
+          exact (orbit_unique hy₀).1 (mem_singleton _) } }
+end
+
+lemma card_fixed_points [fintype S] : fincard' (fixed_points μ) = 
+  let p := λ s : set S, fincard' s ≤ 1 in
+  ∑' o in { o ∈ orbits μ | p o }, fincard' o := 
+begin
+  dsimp only,
+  rw @finsum_const_nat (set S) (by apply_instance) _ 1 _,
+    { rw mul_one,
+      exact fincard.of_equiv (equiv.of_bijective _ $ bijective_map_singleton μ) },
+    { exact λ x ⟨hx₀, hx₁⟩, card_orbits_eq_one hx₀ hx₁ },
+end
+
+lemma card_set_eq_card_fixed_points_sum_card_orbits [fintype S] (μ : laction G S): 
+  fincard' S = fincard' (fixed_points μ) 
+             + let p := λ s : set S, fincard' s ≤ 1 in
+             ∑' o in { o ∈ (orbits μ) | ¬ p o }, fincard' o := 
+begin
+  rw [card_fixed_points, fincard.finsum_in_filter],
+  exact sum_card_orbits.symm
+end
+
+-- I don't think this is needed anymore
+lemma pow_prime_eq_one_or_dvd_prime {p d n : ℕ} (hp: p.prime) (hd: d = p^n) : 
+  d = 1 ∨ p ∣ d := 
+begin
+  cases n,
+  left, rw hd, refl,
+  right, simp [hd, nat.succ_eq_add_one, nat.pow_succ]
+end
+
+-- Are these names okay? Should I leave these lemmas here?
+lemma card_orbit_div_pow_p [fintype S] [fintype G] (μ : laction G S)
+  (p : ℕ) (hp : p.prime) (n : ℕ) (hG : fincard' G = p ^ n):
+  ∀ s : S, fincard'( orbit μ s ) ∣ p^n :=
+begin
+  intro s, rw ← hG,
+    use (fincard' (stabilizer μ s)),
+    rw laction.orbit_stabilizer,
+end  
+
+lemma card_orbit_eq_one_or_dvd_p [fintype S] [fintype G] (μ : laction G S) 
+  (p : ℕ) (hp : p.prime) (n : ℕ) (hG : fincard' G = p ^ n) : 
+  ∀ (s : S), fincard' (orbit μ s) = 1 ∨ p ∣ fincard' (orbit μ s) :=
+begin
+  intro s,
+  cases (card_orbit_div_pow_p μ p hp n hG) s with _ _,
+  have h1: fincard' ↥(orbit μ s) ∣ p^n,
+    { use w, exact h },
+  rw nat.dvd_prime_pow hp at h1,
+  rcases h1 with ⟨_ | a, _, ha⟩; rw ha,
+    { rw nat.pow_zero, left, refl },
+    { right, rw nat.pow_succ, use p ^ a, rw mul_comm }
+end  
+
+lemma card_set_congr_card_fixed_points_mod_prime [fintype S] [fintype G]
+  (μ : laction G S) (p : ℕ) (hp : p.prime) (n : ℕ) (hG : fincard' G = p ^ n) :
+  fincard' S ≡ fincard' (fixed_points μ) [MOD p] := 
+begin
+  rw card_set_eq_card_fixed_points_sum_card_orbits μ,
+  refine nat.modeq.modeq_of_dvd _,
+  suffices: ↑p ∣ ↑∑' (o : set S) in 
+    ({ o ∈ orbits μ | 1 < fincard' o } : set (set S)), fincard' o,
+    { simpa [sub_eq_add_neg] },
+  norm_cast, apply fincard.finsum_divisible_by,
+  rintro x h,
+  rcases h with ⟨⟨s, hs⟩, hr⟩,
+  change x = orbit μ s at hs,
+  rw hs, cases card_orbit_eq_one_or_dvd_p μ p hp n hG s,
+  rw [hs, h] at hr,
+  linarith, assumption
+end
+
+-- Given a subset H of a group G, its conjugate is also a subgroup of G
+def conjugate_subgroup [group G] (g : G) (H : subgroup G) :  subgroup G :=
+{ carrier := { k| ∃ h ∈ H, k = g * h * g⁻¹ },
+  one_mem' := ⟨(1 : G), H.one_mem, by rw [group.mul_one, group.mul_right_inv]⟩,
+  mul_mem' := λ x y ⟨s, hs, h1⟩ ⟨t, ht, h2⟩, 
+    ⟨s * t, H.mul_mem hs ht, by rw [h1, h2]; simp [group.mul_assoc]⟩,
+  inv_mem' := λ x ⟨s, hs, hx⟩, ⟨s⁻¹, H.inv_mem hs, 
+    group.inv_eq_of_mul_eq_one (by rw hx; simp [group.mul_assoc])⟩ }
+
+lemma conjugate_is_conjugate (g : G) (H : subgroup G) : 
+  is_conjugate H (conjugate_subgroup g H) :=
+begin
+  refine ⟨g⁻¹, _⟩, ext x,
+  apply exists_congr,
+  simp [conjugate_subgroup],
+end
+
+lemma mul_equiv_of_is_conjugate {H K : subgroup G} (e : is_conjugate H K) :
+ H ≃* K :=
+let ⟨g, hg⟩ := classical.indefinite_description _ e in
+begin
+  dsimp at hg,
+  rw ext_iff at hg,
+  change ∀ x : G, (∃ (h : G), _) ↔ x ∈ K at hg,
+  exact 
+  { to_fun := λ h, ⟨g⁻¹ * h * g, show _ ∈ K, 
+      begin rw ←hg, use [h.1, h.2], refl end⟩,
+    inv_fun := λ k, ⟨g * k.1 * g⁻¹, 
+      begin 
+        show _ ∈ H, cases k with k hk,
+        rcases (hg k).2 hk with ⟨t, h1, h2⟩,
+        convert h1, subst h2, simp [group.mul_assoc],
+      end⟩,
+    left_inv := λ ⟨_, _⟩, by simp [group.mul_assoc],
+    right_inv := λ ⟨_, _⟩, by simp [group.mul_assoc],
+    map_mul' := λ ⟨_, _⟩ ⟨_, _⟩, by ext; simp [group.mul_assoc] } 
+end
+
+def conjugation_action [group G]: laction G (subgroup G) :=
+{ to_fun := λ (g : G) (H : subgroup G), conjugate_subgroup g H,
+  map_one' := 
+    begin
+      intro H,
+      unfold conjugate_subgroup,
+      norm_num, ext, split,
+      repeat { intro hx, exact hx },         
+    end  ,
+  map_assoc' := 
+    begin
+      intros s t H,
+      ext, split, unfold conjugate_subgroup,
+        { intro hx,
+          rcases hx with ⟨h, ⟨⟨k, ⟨j, hj⟩⟩, h2⟩⟩, 
+          rw hj at h2,
+          suffices: x = s * t * k * (t⁻¹ * s⁻¹), tidy,
+          rw [← group.mul_assoc, h2, group.mul_assoc],
+          apply group.mul_eq_of_eq_inv_mul,
+          symmetry,
+          iterate 4 { rw ← group.mul_assoc },
+          rw [group.mul_left_inv, group.one_mul] },
+        { intro hx,
+          rcases hx with ⟨h, ⟨hh, hj⟩⟩,
+          suffices: x ∈ conjugate_subgroup s (conjugate_subgroup t H), tidy,
+          rw [← group.mul_assoc, ← group.mul_assoc, group.mul_assoc],
+          assumption },
+    end }
+
+-- The normalizer of a subset of G is a subgroup of G 
+def normalizer (A : set G) : subgroup G := 
+{ carrier := { g : G | ∀ n, n ∈ A ↔ g * n * g⁻¹ ∈ A },
+  one_mem' := by intro a; rw [group.one_mul, group.one_inv, group.mul_one],
+  mul_mem' := λ _ _ hx hy _, by rw [hy, hx]; simp [group.mul_assoc],
+  inv_mem' := λ x hx a, by rw hx (x⁻¹ * a * x⁻¹⁻¹); simp [group.mul_assoc] }
+
+lemma mem_normalizer_iff [group G] {H : subgroup G} (x : G):
+  x ∈ normalizer H.carrier ↔ ∀ k : G, k ∈ H ↔ x * k * x⁻¹ ∈ H := by refl
+
+end mygroup
